field_ptr_after

src/3d/prelude/buffer/EverParse3d.Actions.All.fst
@@ -3,6 +3,8 @@ friend EverParse3d.Actions.Base
 friend EverParse3d.InputStream.All
 friend EverParse3d.InputStream.Buffer
 
+let _ = EverParse3d.Actions.BackendFlagValue.backend_flag_value
+
 module IB = EverParse3d.InputBuffer
 module P = EverParse3d.Prelude
 
@@ -13,6 +15,10 @@ let action_field_ptr
    = fun ctxt input startPosition _ ->
        let open LowParse.Slice in
        IB.offset input.EverParse3d.InputStream.Buffer.Aux.buf (LowParse.Low.ErrorCode.uint64_to_uint32 startPosition) input.EverParse3d.InputStream.Buffer.Aux.perm_of
+
+let action_field_ptr_after
+      #nz #wk (#k:P.parser_kind nz wk) (#t:Type) (#p:P.parser k t) n
+   = false_elim ()
 
 let action_field_pos_32
       #nz #wk (#k:P.parser_kind nz wk) (#t:Type) (#p:P.parser k t) (u:unit)
